### 22. Extremum


#### 1. The profit function is $P(u) = -2u^2 + 50u - 300$, where $u$ is the number of units sold. Find the number of units that maximize profit.
 
The formula for the $u$-coordinate of the vertex is given by:  
$u = -\frac{b}{2a}$,  where $P(u) = au^2 + bu + c$. We don't use the quadratic formula because this is only to find 
the roots, weuseonly the first term of that formula because â€‹represents the u-coordinate of the vertex.

Here, $a = -2$, $b = 50$, and $c = -300$. Substituting:  
$u = -\frac{50}{2(-2)} = \frac{50}{4} = 12.5$.

The number of units that maximize profit is 12.5 units.



#### 2. You have 10 meters of string, and you need to use it to enclose the largest possible rectangle. Find the dimensions of the rectangle.

The perimeter is $2x + 2y = 10 = x + y = 5$. The area of the rectangle is $A = x \cdot y$.

Now, we substitute $x = 5 - y$ into $A$:  
$A(y) = (5 - y)y = 5y - y^2$.

We take the derivative of $A(x)$ and then equalize to 0:  
$A'(y) = 5 - 2y = 0 \implies y = 2.5$.

When $y = 2.5$, $y = 5 - 2.5 = 2.5$.  

The dimensions of the rectangle are 2.5mx2.5m. It's not a rectangle, it's a square



#### 3. Find the extremum of $f(x) = x^2 + 3x - 5$.

Its extremum is a minimum, which occurs at the vertex, so we use the formula:  
$x = -\frac{b}{2a}$, where $a = 1, b = 3. c = -5$.  

Substitute:  
$x = -\frac{3}{2(1)} = -\frac{3}{2}$. Now we substitute in the inicial equation.

The minimum value is:  
$f(-\frac{3}{2}) = (-\frac{3}{2})^2 + 3(-\frac{3}{2}) - 5 = \frac{9}{4} - \frac{9}{2} - 5 = -\frac{29}{4}$.

The minimum occurs at $x = -\frac{3}{2}$, with a value of $f(x) = -\frac{29}{4}$.



#### 4. Find the extremum of $f(x) = \frac{x^2 + 2x + 1}{x - 1}$.

 
First, we have to rewrite the function:  
$f(x) = \frac{(x + 1)^2}{x - 1}$.

We calculate $f'(x)$:  
$f'(x) = \frac{(x - 1) \cdot 2(x + 1) - (x + 1)^2 \cdot 1}{(x - 1)^2} = \frac{2(x + 1)(x - 1) - (x + 1)^2}{(x - 1)^2}$.

Simplify the numerator and equalize to 0:  
$2(x + 1)(x - 1) - (x + 1)^2 = 2(x^2 - 1) - (x^2 + 2x + 1) = 2x^2 - 2 - x^2 - 2x - 1 = x^2 - 2x - 3$.
 
$f'(x) = \frac{x^2 - 2x - 3}{(x - 1)^2}$.

$x^2 - 2x - 3 = 0 = (x - 3)(x + 1) = 0 \implies x = 3$ or $x = -1$.


- At $x = 3$: $f(3) = \frac{(3 + 1)^2}{3 - 1} = \frac{16}{2} = 8$.  
- At $x = -1$: $f(-1) = \frac{((-1) + 1)^2}{-1 - 1} = \frac{0}{-2} = 0$.

$f(x)$ has a **maximum** at $x = 3$ with $f(3) = 8$ and a **minimum** at $x = -1$ with $f(-1) = 0$.
