## 25. Differential Equations

1. Solve the following first-order ordinary differential equations:
   - $y'(x)= y$
First, we rewrite the differential equation:  $\frac {dy}{dx} = y$

As we have in the equation y'(x). We use the form of the differential equation as:  $\frac {1 dy}{y} = dx$

We integrate the TWO sides and solve the equation for y by the rule of $ln(x) = y --> x=e^y$:  $\int \frac {1}{y} dy = \int 1 dx --> ln|y| = x + C$

$y = Ce^x$


   - $y'(x) = \frac{1}{2y(x)}$
 First, we rewrite the differential equation and solve the variables: $y\frac {dy}{dx} = \frac {1}{2}$

$2y\frac {dy}{dx} = 1 --> 2ydy = dx$

We integrate the TWO sides: $\int 2y dy = \int 1 dx --> 2\int y dy = \int 1 dx --> y^2= \frac {x}{2} + C$

Solve the equation: $y = \+- \sqrt {\frac {x}{2} + C}$



2. Solve the first-order ordinary differential equations using the method of separation of variables for $x$ and $y=y(x)$:

   - $\frac{dy}{dx} = \frac{x}{y}$
First, we rewrite the differential equation and as the variables are separated, we don't have to do it $y dy = x dx$

We integrate the two sides: $\int y dy = \int x dx$

$\frac {y^2}{2} = \frac {x^2}{2} + C$ and simplify $y = \+- \sqrt {x^2 + 2C}$


   - $\frac{dy}{dx} = \frac{y}{x}$
First, we rewrite the differential equation: $\frac {dy}{y} = \frac {dx}{x}$

Then we integrate the two sides and solve: $\int \frac {1}{y} dy = \int \frac {1}{x} dx --> ln|y| = ln|x| + C --> e^{ln|y|} = e^{ln|x| + C}$

Using exponential rules: $|y| = |x|C --> y = Cx$


   - $\frac{dy}{dx} = xy$
First, we rewrite the differential equation: $\frac {dy}{y} = x dx$

Then we integrate the two sides: $\int \frac {1}{y} dy = \int x dx --> ln|y|= = \frac {x^2}{2}  + C$

$y = Ce^(\frac {x^2}{2})



3. Solve the second-order ordinary differential equations:

   * $y''(x) + y'(x) = 0$, with boundary conditions $y(0) = 2$ and $y'(0) = -1$
We assume a solution of $y = e^{rx}$ where r is the constant. So, $y'' = r^2e^{rx} and y' = re^{rx}$

We substitute: $r^2e^{rx} + re^{rx} --> e^{rx}(r^2 + r) = 0$ and as $e^{rx}$ is different from 0: $r^2 + r = 0$ which solution s $r = 0$ and $r = -1$

Using this solutions: $y(x) = C1e^{0x} + C2e^{-1x} --> y(x) = C1 + C2e^-x$

Now we use the boundary conditions to find C1 and C2:

	- For $y(0) = 2. y(x) = C1 + C2e^0 --> C1 + C2 = 2$
	- For $y'(0) = -1$. The derivative of the constant C1 is 0, so: $y'(x)= 0 + C2 \cdot (-e^-x) --> y'(0) = -C2e^0 --> -C2 = -1 --> C2 = 1$

If $C2 = 1 --> C1 + 1 = 2 --> C1 = 1$

Substitute C1 and C2 in $y(x) = C1 + C2e^-x --> y(x) = 1 + e^-x$


   * $y''(x) - y(x)= 0$, with boundary conditions $y(0) = 2$ and $y'(0) = 0$
$y'' = r^2e^{rx} and y' = e^{rx}$

We solve it: $r^2 - 1= 0 --> (r - 1)(r + 1) = 0 --> r = 1 and r = -1$

Now we substitute he r: $y(x) = C1e^{x} + C2e^{-x}$


Now we use the boundary conditions to find C1 and C2:

	- For $y(0) = 2. y(x) = C1e^0 + C2e^0 --> C1 + C2 = 2$
	- For $y'(0) = 0$. $y'(x)= C1e^x - C2e^-x --> C1 - C2 = 0 --> C1 = C2$

$C1 + C2 = 2 --> 2C1 = 2 --> C1 = 1 and C2 = 1$

Substitute C1 and C2 in $y(x) = C1e^x + C2e^-x --> y(x) = e^x + e^-x$


   * $\frac{d^2\,y(x)}{dx^2} = -\omega^2 y(x)$.
$y'' = r^2e^{rx}$ and substitute in the equation $r^2e^{rx} = -w^2e^{rx} --> r^2 + w^2 = 0 --> r = \+- iw$

Using Euler's formula: $e^{wx} = cos (x) + isin (x)$ we have $y(x) = C1cos(wx) + C2sin(wx)$


4. Check if the function $\psi(t, x) = A \cos(\omega t + kx)$ is a solution of the second-order partial differential equation (the so-called "wave equation"), where $v = \frac{\omega}{k} = \frac{2\pi / T}{2\pi / \lambda}$:

$$
\frac{\partial^2 \psi(t, x)}{\partial t^2} - v^2 \frac{\partial^2 \psi(t, x)}{\partial x^2} = 0.
$$
First, the first partial derivative respect to t: $\frac {\partial\psi}{\partial t} = -A\omega \sin(\omega t + kx)$

Second partial derivative respect t: $\frac {\partial^2 \psi}{\partial t^2} = -A\omega^2\cos(\omega t + kx)$

First partial derivative respect to x: $\frac {\partial\psi}{\partial x} = -Ak\sin(\omega t + kx)$

Second partial derivative respect to x: $\frac {\partial^2 \psi}{\partial x^2} = -Ak^2\cos(\omega t + kx)$

We substitute the second partial derivatives in the wave equation: $-A\omega^2\cos(\omega t + kx) - v^2(-Ak^2\cos(\omega t + kx))$

As $v = \frac {w}{k} then v^2 = \frac {w^2}{k^2}$ and $-A\omega^2\cos(\omega t + kx) + Ak^2\cos(\omega t + kx)$ so 0=0

The function is a solution to the wave equation.








